HOL/Lambda: converted into new-style theory and document;

src/HOL/Lambda/Eta.thy
@@ -2,33 +2,250 @@
     ID:         $Id$
     Author:     Tobias Nipkow
     Copyright   1995 TU Muenchen
-
-Eta-reduction and relatives.
 *)
 
-Eta = ParRed +
-consts free :: dB => nat => bool
-       decr :: dB => dB
-       eta  :: "(dB * dB) set"
+header {* Eta-reduction *}
 
-syntax  "-e>", "-e>>", "-e>=" , "->=" :: [dB,dB] => bool (infixl 50)
+theory Eta = ParRed:
 
-translations
-  "s -e>  t" == "(s,t) : eta"
-  "s -e>> t" == "(s,t) : eta^*"
-  "s -e>= t" == "(s,t) : eta^="
-  "s ->=  t" == "(s,t) : beta^="
 
+subsection {* Definition of eta-reduction and relatives *}
+
+consts
+  free :: "dB => nat => bool"
 primrec
-  "free (Var j) i = (j=i)"
-  "free (s $ t) i = (free s i | free t i)"
-  "free (Abs s) i = free s (i+1)"
+  "free (Var j) i = (j = i)"
+  "free (s $ t) i = (free s i \<or> free t i)"
+  "free (Abs s) i = free s (i + 1)"
+
+consts
+  eta :: "(dB \<times> dB) set"
+
+syntax 
+  "_eta" :: "[dB, dB] => bool"   (infixl "-e>" 50)
+  "_eta_rtrancl" :: "[dB, dB] => bool"   (infixl "-e>>" 50)
+  "_eta_reflcl" :: "[dB, dB] => bool"   (infixl "-e>=" 50)
+translations
+  "s -e> t" == "(s,t) \<in> eta"
+  "s -e>> t" == "(s,t) \<in> eta^*"
+  "s -e>= t" == "(s,t) \<in> eta^="
 
 inductive eta
-intrs
-   eta  "~free s 0 ==> Abs(s $ Var 0) -e> s[dummy/0]"
-   appL  "s -e> t ==> s$u -e> t$u"
-   appR  "s -e> t ==> u$s -e> u$t"
-   abs   "s -e> t ==> Abs s -e> Abs t"
-end
+  intros [simp, intro]
+    eta: "\<not> free s 0 ==> Abs (s $ Var 0) -e> s[dummy/0]"
+    appL: "s -e> t ==> s $ u -e> t $ u"
+    appR: "s -e> t ==> u $ s -e> u $ t"
+    abs: "s -e> t ==> Abs s -e> Abs t"
 
+inductive_cases eta_cases [elim!]:
+  "Abs s -e> z"
+  "s $ t -e> u"
+  "Var i -e> t"
+
+
+subsection "Properties of eta, subst and free"
+
+lemma subst_not_free [rulify, simp]:
+    "\<forall>i t u. \<not> free s i --> s[t/i] = s[u/i]"
+  apply (induct_tac s)
+    apply (simp_all add: subst_Var)
+  done
+
+lemma free_lift [simp]:
+    "\<forall>i k. free (lift t k) i =
+      (i < k \<and> free t i \<or> k < i \<and> free t (i - 1))"
+  apply (induct_tac t)
+    apply (auto cong: conj_cong)
+  apply arith
+  done
+
+lemma free_subst [simp]:
+    "\<forall>i k t. free (s[t/k]) i =
+      (free s k \<and> free t i \<or> free s (if i < k then i else i + 1))"
+  apply (induct_tac s)
+    prefer 2
+    apply simp
+    apply blast
+   prefer 2
+   apply simp
+  apply (simp add: diff_Suc subst_Var split: nat.split)
+  apply clarify
+  apply (erule linorder_neqE)
+  apply simp_all
+  done
+
+lemma free_eta [rulify]:
+    "s -e> t ==> \<forall>i. free t i = free s i"
+  apply (erule eta.induct)
+     apply (simp_all cong: conj_cong)
+  done
+
+lemma not_free_eta:
+    "[| s -e> t; \<not> free s i |] ==> \<not> free t i"
+  apply (simp add: free_eta)
+  done
+
+lemma eta_subst [rulify, simp]:
+    "s -e> t ==> \<forall>u i. s[u/i] -e> t[u/i]"
+  apply (erule eta.induct)
+  apply (simp_all add: subst_subst [symmetric])
+  done
+
+
+subsection "Confluence of eta"
+
+lemma square_eta: "square eta eta (eta^=) (eta^=)"
+  apply (unfold square_def id_def)
+  apply (rule impI [THEN allI [THEN allI]])
+  apply simp
+  apply (erule eta.induct)
+     apply (slowsimp intro: subst_not_free eta_subst free_eta [THEN iffD1])
+    apply safe
+       prefer 5
+       apply (blast intro!: eta_subst intro: free_eta [THEN iffD1])
+      apply blast+
+  done
+
+theorem eta_confluent: "confluent eta"
+  apply (rule square_eta [THEN square_reflcl_confluent])
+  done
+
+
+subsection "Congruence rules for eta*"
+
+lemma rtrancl_eta_Abs: "s -e>> s' ==> Abs s -e>> Abs s'"
+  apply (erule rtrancl_induct)
+   apply (blast intro: rtrancl_refl rtrancl_into_rtrancl)+
+  done
+
+lemma rtrancl_eta_AppL: "s -e>> s' ==> s $ t -e>> s' $ t"
+  apply (erule rtrancl_induct)
+   apply (blast intro: rtrancl_refl rtrancl_into_rtrancl)+
+  done
+
+lemma rtrancl_eta_AppR: "t -e>> t' ==> s $ t -e>> s $ t'"
+  apply (erule rtrancl_induct)
+   apply (blast intro: rtrancl_refl rtrancl_into_rtrancl)+
+  done
+
+lemma rtrancl_eta_App:
+    "[| s -e>> s'; t -e>> t' |] ==> s $ t -e>> s' $ t'"
+  apply (blast intro!: rtrancl_eta_AppL rtrancl_eta_AppR intro: rtrancl_trans)
+  done
+
+
+subsection "Commutation of beta and eta"
+
+lemma free_beta [rulify]:
+    "s -> t ==> \<forall>i. free t i --> free s i"
+  apply (erule beta.induct)
+     apply simp_all
+  done
+
+lemma beta_subst [rulify, intro]:
+    "s -> t ==> \<forall>u i. s[u/i] -> t[u/i]"
+  apply (erule beta.induct)
+     apply (simp_all add: subst_subst [symmetric])
+  done
+
+lemma subst_Var_Suc [simp]: "\<forall>i. t[Var i/i] = t[Var(i)/i + 1]"
+  apply (induct_tac t)
+  apply (auto elim!: linorder_neqE simp: subst_Var)
+  done
+
+lemma eta_lift [rulify, simp]:
+    "s -e> t ==> \<forall>i. lift s i -e> lift t i"
+  apply (erule eta.induct)
+     apply simp_all
+  done
+
+lemma rtrancl_eta_subst [rulify]:
+    "\<forall>s t i. s -e> t --> u[s/i] -e>> u[t/i]"
+  apply (induct_tac u)
+    apply (simp_all add: subst_Var)
+    apply (blast intro: r_into_rtrancl)
+   apply (blast intro: rtrancl_eta_App)
+  apply (blast intro!: rtrancl_eta_Abs eta_lift)
+  done
+
+lemma square_beta_eta: "square beta eta (eta^*) (beta^=)"
+  apply (unfold square_def)
+  apply (rule impI [THEN allI [THEN allI]])
+  apply (erule beta.induct)
+     apply (slowsimp intro: r_into_rtrancl rtrancl_eta_subst eta_subst)
+    apply (blast intro: r_into_rtrancl rtrancl_eta_AppL)
+   apply (blast intro: r_into_rtrancl rtrancl_eta_AppR)
+  apply (slowsimp intro: r_into_rtrancl rtrancl_eta_Abs free_beta
+    other: dB.distinct [iff del, simp])    (*23 seconds?*)
+  done
+
+lemma confluent_beta_eta: "confluent (beta \<union> eta)"
+  apply (assumption |
+    rule square_rtrancl_reflcl_commute confluent_Un
+      beta_confluent eta_confluent square_beta_eta)+
+  done
+
+
+subsection "Implicit definition of eta"
+
+text {* @{term "Abs (lift s 0 $ Var 0) -e> s"} *}
+
+lemma not_free_iff_lifted [rulify]:
+    "\<forall>i. (\<not> free s i) = (\<exists>t. s = lift t i)"
+  apply (induct_tac s)
+    apply simp
+    apply clarify
+    apply (rule iffI)
+     apply (erule linorder_neqE)
+      apply (rule_tac x = "Var nat" in exI)
+      apply simp
+     apply (rule_tac x = "Var (nat - 1)" in exI)
+     apply simp
+    apply clarify
+    apply (rule notE)
+     prefer 2
+     apply assumption
+    apply (erule thin_rl)
+    apply (case_tac t)
+      apply simp
+     apply simp
+    apply simp
+   apply simp
+   apply (erule thin_rl)
+   apply (erule thin_rl)
+   apply (rule allI)
+   apply (rule iffI)
+    apply (elim conjE exE)
+    apply (rename_tac u1 u2)
+    apply (rule_tac x = "u1 $ u2" in exI)
+    apply simp
+   apply (erule exE)
+   apply (erule rev_mp)
+   apply (case_tac t)
+     apply simp
+    apply simp
+    apply blast
+   apply simp
+  apply simp
+  apply (erule thin_rl)
+  apply (rule allI)
+  apply (rule iffI)
+   apply (erule exE)
+   apply (rule_tac x = "Abs t" in exI)
+   apply simp
+  apply (erule exE)
+  apply (erule rev_mp)
+  apply (case_tac t)
+    apply simp
+   apply simp
+  apply simp
+  apply blast
+  done
+
+theorem explicit_is_implicit:
+  "(\<forall>s u. (\<not> free s 0) --> R (Abs (s $ Var 0)) (s[u/0])) =
+    (\<forall>s. R (Abs (lift s 0 $ Var 0)) s)"
+  apply (auto simp add: not_free_iff_lifted)
+  done
+
+end
