src/HOL/Lambda/Lambda.thy
@@ -2,56 +2,205 @@
     ID:         $Id$
     Author:     Tobias Nipkow
     Copyright   1995 TU Muenchen
-
-Lambda-terms in de Bruijn notation,
-substitution and beta-reduction.
 *)
 
-Lambda = Main +
+header {* Basic definitions of Lambda-calculus *}
 
-datatype dB = Var nat | "$" dB dB (infixl 200) | Abs dB
+theory Lambda = Main:
+
+
+subsection {* Lambda-terms in de Bruijn notation and substitution *}
+
+datatype dB =
+    Var nat
+  | App dB dB (infixl "$" 200)
+  | Abs dB
 
 consts
-  subst  :: [dB,dB,nat]=>dB ("_[_'/_]" [300,0,0] 300)
-  lift   :: [dB,nat] => dB
-  (* optimized versions *)
-  substn :: [dB,dB,nat] => dB
-  liftn  :: [nat,dB,nat] => dB
+  subst :: "[dB, dB, nat] => dB"  ("_[_'/_]" [300, 0, 0] 300)
+  lift :: "[dB, nat] => dB"
 
 primrec
-  "lift (Var i) k = (if i < k then Var i else Var(i+1))"
-  "lift (s $ t) k = (lift s k) $ (lift t k)"
-  "lift (Abs s) k = Abs(lift s (k+1))"
+  "lift (Var i) k = (if i < k then Var i else Var (i + 1))"
+  "lift (s $ t) k = lift s k $ lift t k"
+  "lift (Abs s) k = Abs (lift s (k + 1))"
+
+primrec  (* FIXME base names *)
+  subst_Var: "(Var i)[s/k] =
+    (if k < i then Var (i - 1) else if i = k then s else Var i)"
+  subst_App: "(t $ u)[s/k] = t[s/k] $ u[s/k]"
+  subst_Abs: "(Abs t)[s/k] = Abs (t[lift s 0 / k+1])"
+
+declare subst_Var [simp del]
+
+text {* Optimized versions of @{term subst} and @{term lift}. *}
+
+consts
+  substn :: "[dB, dB, nat] => dB"
+  liftn :: "[nat, dB, nat] => dB"
 
 primrec
-  subst_Var "(Var i)[s/k] = (if k < i then Var(i-1)
-                            else if i = k then s else Var i)"
-  subst_App "(t $ u)[s/k] = t[s/k] $ u[s/k]"
-  subst_Abs "(Abs t)[s/k] = Abs (t[lift s 0 / k+1])"
+  "liftn n (Var i) k = (if i < k then Var i else Var (i + n))"
+  "liftn n (s $ t) k = liftn n s k $ liftn n t k"
+  "liftn n (Abs s) k = Abs (liftn n s (k + 1))"
 
 primrec
-  "liftn n (Var i) k = (if i < k then Var i else Var(i+n))"
-  "liftn n (s $ t) k = (liftn n s k) $ (liftn n t k)"
-  "liftn n (Abs s) k = Abs(liftn n s (k+1))"
+  "substn (Var i) s k =
+    (if k < i then Var (i - 1) else if i = k then liftn k s 0 else Var i)"
+  "substn (t $ u) s k = substn t s k $ substn u s k"
+  "substn (Abs t) s k = Abs (substn t s (k + 1))"
 
-primrec
-  "substn (Var i) s k = (if k < i then Var(i-1)
-                         else if i = k then liftn k s 0 else Var i)"
-  "substn (t $ u) s k = (substn t s k) $ (substn u s k)"
-  "substn (Abs t) s k = Abs (substn t s (k+1))"
 
-consts  beta :: "(dB * dB) set"
+subsection {* Beta-reduction *}
 
-syntax  "->", "->>" :: [dB,dB] => bool (infixl 50)
+consts
+  beta :: "(dB \<times> dB) set"
 
+syntax
+  "_beta" :: "[dB, dB] => bool"  (infixl "->" 50)
+  "_beta_rtrancl" :: "[dB, dB] => bool"  (infixl "->>" 50)
 translations
-  "s -> t"  == "(s,t) : beta"
-  "s ->> t" == "(s,t) : beta^*"
+  "s -> t" == "(s,t) \<in> beta"
+  "s ->> t" == "(s,t) \<in> beta^*"
 
 inductive beta
-intrs
-   beta  "(Abs s) $ t -> s[t/0]"
-   appL  "s -> t ==> s$u -> t$u"
-   appR  "s -> t ==> u$s -> u$t"
-   abs   "s -> t ==> Abs s -> Abs t"
+  intros [simp, intro!]
+    beta: "Abs s $ t -> s[t/0]"
+    appL: "s -> t ==> s $ u -> t $ u"
+    appR: "s -> t ==> u $ s -> u $ t"
+    abs: "s -> t ==> Abs s -> Abs t"
+
+inductive_cases beta_cases [elim!]:
+  "Var i -> t"
+  "Abs r -> s"
+  "s $ t -> u"
+
+declare if_not_P [simp] not_less_eq [simp]
+  -- {* don't add @{text "r_into_rtrancl[intro!]"} *}
+
+
+subsection {* Congruence rules *}
+
+lemma rtrancl_beta_Abs [intro!]:
+    "s ->> s' ==> Abs s ->> Abs s'"
+  apply (erule rtrancl_induct)
+   apply (blast intro: rtrancl_into_rtrancl)+
+  done
+
+lemma rtrancl_beta_AppL:
+    "s ->> s' ==> s $ t ->> s' $ t"
+  apply (erule rtrancl_induct)
+   apply (blast intro: rtrancl_into_rtrancl)+
+  done
+
+lemma rtrancl_beta_AppR:
+    "t ->> t' ==> s $ t ->> s $ t'"
+  apply (erule rtrancl_induct)
+   apply (blast intro: rtrancl_into_rtrancl)+
+  done
+
+lemma rtrancl_beta_App [intro]:
+    "[| s ->> s'; t ->> t' |] ==> s $ t ->> s' $ t'"
+  apply (blast intro!: rtrancl_beta_AppL rtrancl_beta_AppR
+    intro: rtrancl_trans)
+  done
+
+
+subsection {* Substitution-lemmas *}
+
+lemma subst_eq [simp]: "(Var k)[u/k] = u"
+  apply (simp add: subst_Var)
+  done
+
+lemma subst_gt [simp]: "i < j ==> (Var j)[u/i] = Var (j - 1)"
+  apply (simp add: subst_Var)
+  done
+
+lemma subst_lt [simp]: "j < i ==> (Var j)[u/i] = Var j"
+  apply (simp add: subst_Var)
+  done
+
+lemma lift_lift [rulify]:
+    "\<forall>i k. i < k + 1 --> lift (lift t i) (Suc k) = lift (lift t k) i"
+  apply (induct_tac t)
+    apply auto
+  done
+
+lemma lift_subst [simp]:
+    "\<forall>i j s. j < i + 1 --> lift (t[s/j]) i = (lift t (i + 1)) [lift s i / j]"
+  apply (induct_tac t)
+    apply (simp_all add: diff_Suc subst_Var lift_lift split: nat.split)
+  done
+
+lemma lift_subst_lt:
+    "\<forall>i j s. i < j + 1 --> lift (t[s/j]) i = (lift t i) [lift s i / j + 1]"
+  apply (induct_tac t)
+    apply (simp_all add: subst_Var lift_lift)
+  done
+
+lemma subst_lift [simp]:
+    "\<forall>k s. (lift t k)[s/k] = t"
+  apply (induct_tac t)
+    apply simp_all
+  done
+
+lemma subst_subst [rulify]:
+    "\<forall>i j u v. i < j + 1 --> t[lift v i / Suc j][u[v/j]/i] = t[u/i][v/j]"
+  apply (induct_tac t)
+    apply (simp_all
+      add: diff_Suc subst_Var lift_lift [symmetric] lift_subst_lt
+      split: nat.split)
+  apply (auto elim: nat_neqE)
+  done
+
+
+subsection {* Equivalence proof for optimized substitution *}
+
+lemma liftn_0 [simp]: "\<forall>k. liftn 0 t k = t"
+  apply (induct_tac t)
+    apply (simp_all add: subst_Var)
+  done
+
+lemma liftn_lift [simp]:
+    "\<forall>k. liftn (Suc n) t k = lift (liftn n t k) k"
+  apply (induct_tac t)
+    apply (simp_all add: subst_Var)
+  done
+
+lemma substn_subst_n [simp]:
+    "\<forall>n. substn t s n = t[liftn n s 0 / n]"
+  apply (induct_tac t)
+    apply (simp_all add: subst_Var)
+  done
+
+theorem substn_subst_0: "substn t s 0 = t[s/0]"
+  apply simp
+  done
+
+
+subsection {* Preservation theorems *}
+
+text {* Not used in Church-Rosser proof, but in Strong
+  Normalization. \medskip *}
+
+theorem subst_preserves_beta [rulify, simp]:
+    "r -> s ==> \<forall>t i. r[t/i] -> s[t/i]"
+  apply (erule beta.induct)
+     apply (simp_all add: subst_subst [symmetric])
+  done
+
+theorem lift_preserves_beta [rulify, simp]:
+    "r -> s ==> \<forall>i. lift r i -> lift s i"
+  apply (erule beta.induct)
+     apply auto
+  done
+
+theorem subst_preserves_beta2 [rulify, simp]:
+    "\<forall>r s i. r -> s --> t[r/i] ->> t[s/i]"
+  apply (induct_tac t)
+    apply (simp add: subst_Var r_into_rtrancl)
+   apply (simp add: rtrancl_beta_App)
+  apply (simp add: rtrancl_beta_Abs)
+  done
+
 end
