src/HOL/Lambda/ParRed.thy
@@ -3,32 +3,131 @@
     Author:     Tobias Nipkow
     Copyright   1995 TU Muenchen
 
-Parallel reduction and a complete developments function "cd".
+Properties of => and "cd", in particular the diamond property of => and
+confluence of beta.
 *)
 
-ParRed = Lambda + Commutation +
+header {* Parallel reduction and a complete developments *}
 
-consts  par_beta :: "(dB * dB) set"
+theory ParRed = Lambda + Commutation:
 
-syntax  "=>" :: [dB,dB] => bool (infixl 50)
 
-translations
-  "s => t" == "(s,t) : par_beta"
-
-inductive par_beta
-  intrs
-    var   "Var n => Var n"
-    abs   "s => t ==> Abs s => Abs t"
-    app   "[| s => s'; t => t' |] ==> s $ t => s' $ t'"
-    beta  "[| s => s'; t => t' |] ==> (Abs s) $ t => s'[t'/0]"
+subsection {* Parallel reduction *}
 
 consts
-  cd  :: dB => dB
+  par_beta :: "(dB \<times> dB) set"
 
-recdef cd "measure size"
-  "cd(Var n) = Var n"
-  "cd(Var n     $ t) = Var n $ cd t"
-  "cd((s1 $ s2) $ t) = cd(s1 $ s2) $ cd t"
-  "cd(Abs u     $ t) = (cd u)[cd t/0]"
-  "cd(Abs s) = Abs(cd s)"
+syntax
+  par_beta :: "[dB, dB] => bool"  (infixl "=>" 50)
+translations
+  "s => t" == "(s, t) \<in> par_beta"
+
+inductive par_beta
+  intros [simp, intro!]
+    var: "Var n => Var n"
+    abs: "s => t ==> Abs s => Abs t"
+    app: "[| s => s'; t => t' |] ==> s $ t => s' $ t'"
+    beta: "[| s => s'; t => t' |] ==> (Abs s) $ t => s'[t'/0]"
+
+inductive_cases par_beta_cases [elim!]:
+  "Var n => t"
+  "Abs s => Abs t"
+  "(Abs s) $ t => u"
+  "s $ t => u"
+  "Abs s => t"
+
+
+subsection {* Inclusions *}
+
+text {* @{text "beta \<subseteq> par_beta \<subseteq> beta^*"} \medskip *}
+
+lemma par_beta_varL [simp]:
+    "(Var n => t) = (t = Var n)"
+  apply blast
+  done
+
+lemma par_beta_refl [simp]: "t => t"  (* par_beta_refl [intro!] causes search to blow up *)
+  apply (induct_tac t)
+    apply simp_all
+  done
+
+lemma beta_subset_par_beta: "beta <= par_beta"
+  apply (rule subsetI)
+  apply clarify
+  apply (erule beta.induct)
+     apply (blast intro!: par_beta_refl)+
+  done
+
+lemma par_beta_subset_beta: "par_beta <= beta^*"
+  apply (rule subsetI)
+  apply clarify
+  apply (erule par_beta.induct)
+     apply blast
+    apply (blast del: rtrancl_refl intro: rtrancl_into_rtrancl)+
+      -- {* @{thm[source] rtrancl_refl} complicates the proof by increasing the branching factor *}
+  done
+
+
+subsection {* Misc properties of par-beta *}
+
+lemma par_beta_lift [rulify, simp]:
+    "\<forall>t' n. t => t' --> lift t n => lift t' n"
+  apply (induct_tac t)
+    apply fastsimp+
+  done
+
+lemma par_beta_subst [rulify]:
+    "\<forall>s s' t' n. s => s' --> t => t' --> t[s/n] => t'[s'/n]"
+  apply (induct_tac t)
+    apply (simp add: subst_Var)
+   apply (intro strip)
+   apply (erule par_beta_cases)
+    apply simp
+   apply (simp add: subst_subst [symmetric])
+   apply (fastsimp intro!: par_beta_lift)
+  apply fastsimp
+  done
+
+
+subsection {* Confluence (directly) *}
+
+lemma diamond_par_beta: "diamond par_beta"
+  apply (unfold diamond_def commute_def square_def)
+  apply (rule impI [THEN allI [THEN allI]])
+  apply (erule par_beta.induct)
+     apply (blast intro!: par_beta_subst)+
+  done
+
+
+subsection {* Complete developments *}
+
+consts
+  "cd" :: "dB => dB"
+recdef "cd" "measure size"
+  "cd (Var n) = Var n"
+  "cd (Var n $ t) = Var n $ cd t"
+  "cd ((s1 $ s2) $ t) = cd (s1 $ s2) $ cd t"
+  "cd (Abs u $ t) = (cd u)[cd t/0]"
+  "cd (Abs s) = Abs (cd s)"
+
+lemma par_beta_cd [rulify]:
+    "\<forall>t. s => t --> t => cd s"
+  apply (induct_tac s rule: cd.induct)
+      apply auto
+  apply (fast intro!: par_beta_subst)
+  done
+
+
+subsection {* Confluence (via complete developments) *}
+
+lemma diamond_par_beta2: "diamond par_beta"
+  apply (unfold diamond_def commute_def square_def)
+  apply (blast intro: par_beta_cd)
+  done
+
+theorem beta_confluent: "confluent beta"
+  apply (rule diamond_par_beta2 diamond_to_confluence
+    par_beta_subset_beta beta_subset_par_beta)+
+  done
+
 end
