src/HOL/Lambda/Commutation.thy
@@ -2,28 +2,137 @@
     ID:         $Id$
     Author:     Tobias Nipkow
     Copyright   1995  TU Muenchen
-
-Abstract commutation and confluence notions.
 *)
 
-Commutation = Main +
+header {* Abstract commutation and confluence notions *}
 
-consts
-  square  :: "[('a*'a)set,('a*'a)set,('a*'a)set,('a*'a)set] => bool"
-  commute :: "[('a*'a)set,('a*'a)set] => bool"
-  confluent, diamond, Church_Rosser :: "('a*'a)set => bool"
+theory Commutation = Main:
 
-defs
-  square_def
- "square R S T U == !x y.(x,y):R --> (!z.(x,z):S --> (? u. (y,u):T & (z,u):U))"
+subsection {* Basic definitions *}
 
-  commute_def "commute R S == square R S S R"
-  diamond_def "diamond R   == commute R R"
+constdefs
+  square :: "[('a \<times> 'a) set, ('a \<times> 'a) set, ('a \<times> 'a) set, ('a \<times> 'a) set] => bool"
+  "square R S T U ==
+    \<forall>x y. (x, y) \<in> R --> (\<forall>z. (x, z) \<in> S --> (\<exists>u. (y, u) \<in> T \<and> (z, u) \<in> U))"
 
-  Church_Rosser_def "Church_Rosser(R) ==   
-  !x y. (x,y) : (R Un R^-1)^* --> (? z. (x,z) : R^* & (y,z) : R^*)"
+  commute :: "[('a \<times> 'a) set, ('a \<times> 'a) set] => bool"
+  "commute R S == square R S S R"
 
+  diamond :: "('a \<times> 'a) set => bool"
+  "diamond R == commute R R"
+
+  Church_Rosser :: "('a \<times> 'a) set => bool"
+  "Church_Rosser R ==
+    \<forall>x y. (x, y) \<in> (R \<union> R^-1)^* --> (\<exists>z. (x, z) \<in> R^* \<and> (y, z) \<in> R^*)"
+
+syntax
+  confluent :: "('a \<times> 'a) set => bool"
 translations
-  "confluent R" == "diamond(R^*)"
+  "confluent R" == "diamond (R^*)"
+
+
+subsection {* Basic lemmas *}
+
+subsubsection {* square *}
+
+lemma square_sym: "square R S T U ==> square S R U T"
+  apply (unfold square_def)
+  apply blast
+  done
+
+lemma square_subset:
+    "[| square R S T U; T \<subseteq> T' |] ==> square R S T' U"
+  apply (unfold square_def)
+  apply blast
+  done
+
+lemma square_reflcl:
+    "[| square R S T (R^=); S \<subseteq> T |] ==> square (R^=) S T (R^=)"
+  apply (unfold square_def)
+  apply blast
+  done
+
+lemma square_rtrancl:
+    "square R S S T ==> square (R^*) S S (T^*)"
+  apply (unfold square_def)
+  apply (intro strip)
+  apply (erule rtrancl_induct)
+   apply blast
+  apply (blast intro: rtrancl_into_rtrancl)
+  done
+
+lemma square_rtrancl_reflcl_commute:
+    "square R S (S^*) (R^=) ==> commute (R^*) (S^*)"
+  apply (unfold commute_def)
+  apply (fastsimp dest: square_reflcl square_sym [THEN square_rtrancl]
+    elim: r_into_rtrancl)
+  done
+
+
+subsubsection {* commute *}
+
+lemma commute_sym: "commute R S ==> commute S R"
+  apply (unfold commute_def)
+  apply (blast intro: square_sym)
+  done
+
+lemma commute_rtrancl: "commute R S ==> commute (R^*) (S^*)"
+  apply (unfold commute_def)
+  apply (blast intro: square_rtrancl square_sym)
+  done
+
+lemma commute_Un:
+    "[| commute R T; commute S T |] ==> commute (R \<union> S) T"
+  apply (unfold commute_def square_def)
+  apply blast
+  done
+
+
+subsubsection {* diamond, confluence, and union *}
+
+lemma diamond_Un:
+    "[| diamond R; diamond S; commute R S |] ==> diamond (R \<union> S)"
+  apply (unfold diamond_def)
+  apply (assumption | rule commute_Un commute_sym)+
+  done
+
+lemma diamond_confluent: "diamond R ==> confluent R"
+  apply (unfold diamond_def)
+  apply (erule commute_rtrancl)
+  done
+
+lemma square_reflcl_confluent:
+    "square R R (R^=) (R^=) ==> confluent R"
+  apply (unfold diamond_def)
+  apply (fast intro: square_rtrancl_reflcl_commute r_into_rtrancl
+    elim: square_subset)
+  done
+
+lemma confluent_Un:
+    "[| confluent R; confluent S; commute (R^*) (S^*) |] ==> confluent (R \<union> S)"
+  apply (rule rtrancl_Un_rtrancl [THEN subst])
+  apply (blast dest: diamond_Un intro: diamond_confluent)
+  done
+
+lemma diamond_to_confluence:
+    "[| diamond R; T \<subseteq> R; R \<subseteq> T^* |] ==> confluent T"
+  apply (force intro: diamond_confluent
+    dest: rtrancl_subset [symmetric])
+  done
+
+
+subsection {* Church-Rosser *}
+
+lemma Church_Rosser_confluent: "Church_Rosser R = confluent R"
+  apply (unfold square_def commute_def diamond_def Church_Rosser_def)
+  apply (tactic {* safe_tac HOL_cs *})
+   apply (tactic {*
+     blast_tac (HOL_cs addIs
+       [Un_upper2 RS rtrancl_mono RS subsetD RS rtrancl_trans,
+       rtrancl_converseI, converseI, Un_upper1 RS rtrancl_mono RS subsetD]) 1 *})
+  apply (erule rtrancl_induct)
+   apply blast
+  apply (blast del: rtrancl_refl intro: r_into_rtrancl rtrancl_trans)
+  done
 
 end
